Task 52 (first steps)

Carleson/DiscreteCarleson.lean
@@ -1,5 +1,6 @@
 import Carleson.Forest
 import Carleson.HardyLittlewood
+import Mathlib.Order.KrullDimension
 -- import Carleson.Proposition2
 -- import Carleson.Proposition3
 
@@ -8,6 +9,127 @@ open scoped ENNReal
 open Classical -- We use quite some `Finset.filter`
 noncomputable section
 
+
+section PartialOrderConstructionWithoutNameSoFar
+
+variable {α} [PartialOrder α] {s : Set α}
+
+-- This operation needs a name.
+-- And maybe easier to define via the height, rather than iteratively?
+
+def foo (s : Set α) (n : ℕ) : Set α := minimals (·≤·) (s \ ⋃ (n' < n), foo s n')
+
+lemma Disjoint_foo {n n'} (h : n ≠ n') : Disjoint (foo s n) (foo (α := α) s n') := by
+  wlog hl : n < n'; · exact (this h.symm (by omega)).symm
+  rw [disjoint_right]; intro p hp
+  rw [foo, mem_minimals_iff, mem_diff] at hp; replace hp := hp.1.2; contrapose! hp
+  refine mem_iUnion₂_of_mem hl hp
+
+lemma PairwiseDisjoint_foo : univ.PairwiseDisjoint (foo s) := fun _ _ _ _ => Disjoint_foo
+
+lemma foo_subset {n : ℕ} : foo s n ⊆ s := calc
+  foo s n = minimals (·≤·) (s \ ⋃ (n' < n), foo s n') := foo.eq_def ..
+  _ ⊆ s \ ⋃ (n' < n), foo s n' := minimals_subset ..
+  _ ⊆ s := diff_subset
+
+-- How do we want to express “has no chains of length n+1”?
+-- Direcly via LTSeries, or via the krullDim?
+
+
+-- Relating minimals and height; base case for the next lemma
+lemma mem_minimals_iff_height_zero {x} (hxs : x ∈ s) :
+    x ∈ minimals (·≤·) s ↔ height s ⟨x, hxs⟩ = 0 := by
+  constructor
+  · intro hx
+    unfold height
+    have : Iic (⟨x, hxs⟩ : s) = {(⟨x, hxs⟩ : s)} := sorry
+    rw [this]
+    apply krullDim_eq_zero_of_unique
+  · intro hx
+    rw [mem_minimals_iff_forall_lt_not_mem]
+    refine ⟨hxs, ?_⟩
+    intros y hyx hys
+    let ls : LTSeries (Iic (⟨x, hxs⟩ : s)) := RelSeries.singleton _ ⟨⟨y, hys⟩, le_of_lt hyx⟩
+    let ls : LTSeries _ := ls.snoc ⟨⟨x, hxs⟩, le_rfl⟩ hyx
+    have : ls.length = 1 := rfl
+    have : 1 ≤ height s ⟨x, hxs⟩ := by
+      apply le_iSup_of_le
+      apply le_of_eq
+      apply symm
+      norm_cast
+    rw [hx] at this
+    contradiction
+
+-- This could show that this construction just partitions by height.
+-- Maybe worth using as the definition (and getting pairwise disjoint for free)?
+-- Or maybe worth avoiding height here altogether, with the `WithBot (WithTop _)` complications?
+lemma mem_foo_iff_height {n : ℕ} {x} (hxs : x ∈ s) :
+  x ∈ foo s n ↔ height s ⟨x, hxs⟩ = n := by
+  induction n generalizing x hxs with
+  | zero =>
+    rw [foo]; simp_rw [not_lt_zero', iUnion_of_empty, iUnion_empty, diff_empty]
+    apply mem_minimals_iff_height_zero
+  | succ n ih =>
+    sorry
+
+
+-- This is generalized from 𝔰 to arbrary f
+-- But maybe more natural would be to say that there is a chain of length `n` that ends in `x`
+-- (which might follow from mem_foo_iff_height)
+lemma exists_le_of_mem_foo {n : ℕ} {x : α} (hx : x ∈ foo s n) (f : α → ℤ) (hf : StrictMono f) :
+    ∃ x' ∈ s, x' ≤ x ∧ f x' + n ≤ f x := by
+  induction n generalizing x with
+  | zero =>
+    rw [foo] at hx; simp_rw [not_lt_zero', iUnion_of_empty, iUnion_empty, diff_empty] at hx
+    use x, hx.1; simp
+  | succ n ih =>
+    have nx : x ∉ foo s n := disjoint_right.mp (Disjoint_foo (by omega)) hx
+    rw [foo, mem_minimals_iff] at hx nx
+    have rl : x ∈ s \ ⋃ (n' < n), foo s n' := by
+      refine mem_of_mem_of_subset hx.1 (diff_subset_diff_right ?_)
+      refine biUnion_subset_biUnion_left fun k hk ↦ ?_
+      rw [mem_def, Nat.le_eq] at hk ⊢; omega
+    simp_rw [rl, true_and] at nx; push_neg at nx; obtain ⟨x', hx', lp⟩ := nx
+    have mp' : x' ∈ foo s n := by
+      by_contra h
+      have cp : x' ∈ s \ ⋃ (n' < n + 1), foo s n' := by
+        have : ∀ n', n' < n + 1 ↔ n' < n ∨ n' = n := by omega
+        simp_rw [this, iUnion_or, iUnion_union_distrib]
+        simp only [iUnion_iUnion_eq_left, mem_diff, mem_union, mem_iUnion, exists_prop, not_or,
+          not_exists, not_and] at hx' ⊢
+        tauto
+      exact absurd (hx.2 cp lp.1) (ne_eq _ _ ▸ lp.2)
+    obtain ⟨d, md, ld, sd⟩ := ih mp'
+    use d, md, (ld.trans lp.1)
+    have hp' : f x' < f x := hf (lt_of_le_of_ne lp.1 lp.2.symm)
+    omega
+
+-- WIP. Unclear what the best formulation for the precondition is
+lemma iUnion_foo {n : ℕ}
+  (hlength : (s : LTSeries s) → s.length ≤ n)
+  -- (hkrull : krullDim α < n)
+  : ⋃ (l ≤ n), foo s l = s := by
+  apply subset_antisymm
+  · apply iUnion_subset
+    intro _
+    apply iUnion_subset
+    intro _
+    apply foo_subset
+  · intro x hx
+    sorry
+
+lemma IsAntichain_foo {n : ℕ}: IsAntichain (·≤·) (foo s n) := by
+  rw [foo]
+  apply minimals_antichain
+
+-- TODO: Define via foo and dual order to get all the nice bits
+def foo' (s : Set α) (n : ℕ) : Set α := maximals (·≤·) (s \ ⋃ (n' < n), foo s n')
+
+lemma IsAntichain_foo' {n : ℕ}: IsAntichain (·≤·) (foo' s n) := by
+  rw [foo']
+  apply maximals_antichain
+
+end PartialOrderConstructionWithoutNameSoFar
 
 open scoped ShortVariables
 variable {X : Type*} {a : ℕ} {q : ℝ} {K : X → X → ℂ} {σ₁ σ₂ : X → ℤ} {F G : Set X}
@@ -76,47 +198,30 @@ Not to be confused with `𝔏₀(k, n, j)` which is called `𝔏₀'` in Lean. -
 def 𝔏₀ (k n : ℕ) : Set (𝔓 X) :=
   { p ∈ ℭ k n | 𝔅 k n p = ∅ }
 
+
 /-- `𝔏₁(k, n, j, l)` consists of the minimal elements in `ℭ₁(k, n, j)` not in
   `𝔏₁(k, n, j, l')` for some `l' < l`. Defined near (5.1.11). -/
 def 𝔏₁ (k n j l : ℕ) : Set (𝔓 X) :=
-  minimals (·≤·) (ℭ₁ k n j \ ⋃ (l' < l), 𝔏₁ k n j l')
+  -- minimals (·≤·) (ℭ₁ k n j \ ⋃ (l' < l), 𝔏₁ k n j l')
+  foo (ℭ₁ k n j) l
 
-lemma 𝔏₁_disjoint {k n j l l' : ℕ} (h : l ≠ l') : Disjoint (𝔏₁ (X := X) k n j l) (𝔏₁ k n j l') := by
-  wlog hl : l < l'; · exact (this h.symm (by omega)).symm
-  rw [disjoint_right]; intro p hp
-  rw [𝔏₁, mem_minimals_iff, mem_diff] at hp; replace hp := hp.1.2; contrapose! hp
-  refine mem_iUnion₂_of_mem hl hp
+lemma 𝔏₁_disjoint {k n j l l' : ℕ} (h : l ≠ l') : Disjoint (𝔏₁ (X := X) k n j l) (𝔏₁ k n j l') :=
+  Disjoint_foo h
+
+/-
+TODO: How to extract this into its own lemma
+
+lemma strict_mono_s : StrictMono 𝔰 := by
+  sorry
+-/
 
 lemma exists_le_of_mem_𝔏₁ {k n j l : ℕ} {p : 𝔓 X} (hp : p ∈ 𝔏₁ k n j l) :
     ∃ p' ∈ ℭ₁ k n j, p' ≤ p ∧ 𝔰 p' + l ≤ 𝔰 p := by
-  induction l generalizing p with
-  | zero =>
-    rw [𝔏₁] at hp; simp_rw [not_lt_zero', iUnion_of_empty, iUnion_empty, diff_empty] at hp
-    use p, hp.1; simp
-  | succ l ih =>
-    have np : p ∉ 𝔏₁ k n j l := disjoint_right.mp (𝔏₁_disjoint (by omega)) hp
-    rw [𝔏₁, mem_minimals_iff] at hp np
-    have rl : p ∈ ℭ₁ k n j \ ⋃ (l' < l), 𝔏₁ k n j l' := by
-      refine mem_of_mem_of_subset hp.1 (diff_subset_diff_right ?_)
-      refine biUnion_subset_biUnion_left fun k hk ↦ ?_
-      rw [mem_def, Nat.le_eq] at hk ⊢; omega
-    simp_rw [rl, true_and] at np; push_neg at np; obtain ⟨p', hp', lp⟩ := np
-    have mp' : p' ∈ 𝔏₁ k n j l := by
-      by_contra h
-      have cp : p' ∈ ℭ₁ k n j \ ⋃ (l' < l + 1), 𝔏₁ k n j l' := by
-        have : ∀ l', l' < l + 1 ↔ l' < l ∨ l' = l := by omega
-        simp_rw [this, iUnion_or, iUnion_union_distrib]
-        simp only [iUnion_iUnion_eq_left, mem_diff, mem_union, mem_iUnion, exists_prop, not_or,
-          not_exists, not_and] at hp' ⊢
-        tauto
-      exact absurd (hp.2 cp lp.1) (ne_eq _ _ ▸ lp.2)
-    obtain ⟨d, md, ld, sd⟩ := ih mp'; use d, md, (ld.trans lp.1)
-    rw [Nat.cast_add, Nat.cast_one, ← add_assoc]
-    have 𝓘lt : 𝓘 p' < 𝓘 p := by
-      refine lt_of_le_of_ne lp.1.1 (not_lt_of_𝓘_eq_𝓘.mt ?_)
-      rw [not_not]; exact lt_of_le_of_ne lp.1 lp.2.symm
-    have 𝔰lt : 𝔰 p' < 𝔰 p := by rw [Grid.lt_def] at 𝓘lt; exact 𝓘lt.2
-    omega
+  refine exists_le_of_mem_foo hp _ ?mono
+  · show StrictMono 𝔰
+    intro p' p hp
+    have 𝓘lt : 𝓘 p' < 𝓘 p := 𝓘_strict_mono hp
+    rw [Grid.lt_def] at 𝓘lt; exact 𝓘lt.2
 
 /-- The subset `ℭ₂(k, n, j)` of `ℭ₁(k, n, j)`, given in (5.1.13). -/
 def ℭ₂ (k n j : ℕ) : Set (𝔓 X) :=
@@ -145,7 +250,7 @@ lemma exists_le_of_mem_ℭ₂ {k n j : ℕ} {p : 𝔓 X} (hp : p ∈ ℭ₂ k n 
     not_and, mem_toFinset] at mp' maxp'
   conv at maxp' => enter [x]; rw [and_imp]
   have mp'₁ : p' ∈ 𝔏₁ k n j (Z * (n + 1)) := by
-    rw [𝔏₁, mem_minimals_iff]
+    rw [𝔏₁, foo, mem_minimals_iff]
     simp_rw [mem_diff, mem_iUnion, exists_prop, not_exists, not_and]
     exact ⟨mp'.1, fun y hy ly ↦ (eq_of_le_of_not_lt ly (maxp' y hy (ly.trans mp'.2))).symm⟩
   obtain ⟨po, mpo, lpo, spo⟩ := exists_le_of_mem_𝔏₁ mp'₁
@@ -171,7 +276,7 @@ lemma ℭ₃_subset_ℭ₂ {k n j : ℕ} : ℭ₃ k n j ⊆ ℭ₂ (X := X) k n 
 /-- `𝔏₃(k, n, j, l)` consists of the maximal elements in `ℭ₃(k, n, j)` not in
   `𝔏₃(k, n, j, l')` for some `l' < l`. Defined near (5.1.17). -/
 def 𝔏₃ (k n j l : ℕ) : Set (𝔓 X) :=
-  maximals (·≤·) (ℭ₃ k n j \ ⋃ (l' < l), 𝔏₃ k n j l')
+  foo' (ℭ₃ k n j) l
 
 /-- The subset `ℭ₄(k, n, j)` of `ℭ₃(k, n, j)`, given in (5.1.19). -/
 def ℭ₄ (k n j : ℕ) : Set (𝔓 X) :=
@@ -964,7 +1069,7 @@ lemma ordConnected_C2 : OrdConnected (ℭ₂ k n j : Set (𝔓 X)) := by
   by_cases e : p = p'; · rwa [e] at mp
   simp_rw [ℭ₂, mem_diff, mp'₁, true_and]
   by_contra h; rw [mem_iUnion₂] at h; obtain ⟨l', bl', p'm⟩ := h
-  rw [𝔏₁, mem_minimals_iff] at p'm
+  rw [𝔏₁, foo, mem_minimals_iff] at p'm
   have pnm : p ∉ ⋃ l'', ⋃ (_ : l'' < l'), 𝔏₁ k n j l'' := by
     replace mp := mp.2; contrapose! mp
     exact mem_of_mem_of_subset mp
@@ -992,7 +1097,7 @@ lemma ordConnected_C4 : OrdConnected (ℭ₄ k n j : Set (𝔓 X)) := by
   by_cases e : p' = p''; · rwa [← e] at mp''
   simp_rw [ℭ₄, mem_diff, mp'₁, true_and]
   by_contra h; simp_rw [mem_iUnion] at h; obtain ⟨l', hl', p'm⟩ := h
-  rw [𝔏₃, mem_maximals_iff] at p'm; simp_rw [mem_diff] at p'm
+  rw [𝔏₃, foo', mem_maximals_iff] at p'm; simp_rw [mem_diff] at p'm
   have p''nm : p'' ∉ ⋃ l'', ⋃ (_ : l'' < l'), 𝔏₃ k n j l'' := by
     replace mp'' := mp''.2; contrapose! mp''
     refine mem_of_mem_of_subset mp'' <| iUnion₂_mono' fun i hi ↦ ⟨i, hi.le.trans hl', subset_rfl⟩
@@ -1484,8 +1589,7 @@ lemma antichain_decomposition : 𝔓pos (X := X) ∩ 𝔓₁ᶜ = ℜ₀ ∪ ℜ
 -- (antichainness, union, the fact that it stops after `n`
 -- steps if there are no antichains of length `n + 1`)
 -- in proper generality.
-def 𝔏₀' (k n l : ℕ) : Set (𝔓 X) :=
-  minimals (·≤·) (𝔏₀ k n \ ⋃ (l' < l), 𝔏₀' k n l')
+def 𝔏₀' (k n l : ℕ) : Set (𝔓 X) := foo (𝔏₀ k n) l
 
 /-- Part of Lemma 5.5.2 -/
 lemma iUnion_L0' : ⋃ (l ≤ n), 𝔏₀' (X := X) k n l = 𝔏₀ k n :=
@@ -1493,11 +1597,11 @@ lemma iUnion_L0' : ⋃ (l ≤ n), 𝔏₀' (X := X) k n l = 𝔏₀ k n :=
 
 /-- Part of Lemma 5.5.2 -/
 lemma pairwiseDisjoint_L0' : univ.PairwiseDisjoint (𝔏₀' (X := X) k n) :=
-  sorry
+  PairwiseDisjoint_foo
 
 /-- Part of Lemma 5.5.2 -/
 lemma antichain_L0' : IsAntichain (·≤·) (𝔏₀' (X := X) k n l) :=
-  sorry
+  IsAntichain_foo
 
 /-- Lemma 5.5.3 -/
 lemma antichain_L2 : IsAntichain (·≤·) (𝔏₂ (X := X) k n j) :=
@@ -1505,11 +1609,11 @@ lemma antichain_L2 : IsAntichain (·≤·) (𝔏₂ (X := X) k n j) :=
 
 /-- Part of Lemma 5.5.4 -/
 lemma antichain_L1 : IsAntichain (·≤·) (𝔏₁ (X := X) k n j l) :=
-  sorry
+  IsAntichain_foo
 
 /-- Part of Lemma 5.5.4 -/
 lemma antichain_L3 : IsAntichain (·≤·) (𝔏₃ (X := X) k n j l) :=
-  sorry
+  IsAntichain_foo'
 
 /-- The constant used in Lemma 5.1.3, with value `2 ^ (210 * a ^ 3) / (q - 1) ^ 5` -/
 -- todo: redefine in terms of other constants
